Test/dafny0/runtest.bat
@@ -20,7 +20,7 @@ for %%f in (BQueue.bpl) do (
 for %%f in (SmallTests.dfy Queue.dfy ListCopy.dfy
             BinaryTree.dfy ListReverse.dfy ListContents.dfy
             SchorrWaite.dfy Termination.dfy Use.dfy DTypes.dfy
-            TypeParameters.dfy) do (
+            TypeParameters.dfy Datatypes.dfy) do (
   echo.
   echo -------------------- %%f --------------------
   %DAFNY_EXE% %* %%f
